@prefix nidm: <http://purl.org/nidash/nidm#> .
@prefix prov: <http://www.w3.org/ns/prov#> .
@prefix rdf: <http://www.w3.org/1999/02/22-rdf-syntax-ns#> .
@prefix rdfs: <http://www.w3.org/2000/01/rdf-schema#> .
@prefix reproschema: <http://schema.repronim.org/> .
@prefix schema: <http://schema.org/> .
@prefix skos: <http://www.w3.org/2004/02/skos/core#> .

reproschema:Activity a nidm:Assessment,
        rdfs:Class,
        prov:Entity,
        prov:Plan ;
    rdfs:label "Activity" ;
    rdfs:comment "An assessment in a protocol." ;
    rdfs:subClassOf schema:CreativeWork .

reproschema:AdditionalNoteObj a rdfs:Class ;
    rdfs:label "Additional Notes Object" ;
    rdfs:comment "A set of objects to define notes in a field. For example, most Redcap and NDA data dictionaries have notes for each item which needs to be captured in reproschema" .

reproschema:AdditionalProperty a rdfs:Class ;
    rdfs:label "Additional properties" ;
    rdfs:comment "An object to describe the various properties added to assessments and fields." .

reproschema:AllowExport a rdfs:Class ;
    rdfs:label "Allow export" ;
    rdfs:comment "Indicates (by boolean) if data can be exported or not." .

reproschema:AllowReplay a rdfs:Class ;
    rdfs:label "Allow replay" ;
    rdfs:comment "Indicates (by boolean) if items can be replayed or not." .

reproschema:AutoAdvance a rdfs:Class ;
    rdfs:label "Auto advance" ;
    rdfs:comment "Indicates (by boolean) if assessments in a protocol can auto advance or not." .

reproschema:Choice a rdfs:Class ;
    rdfs:label "Response choice" ;
    rdfs:comment "An object to describe a response option." .

reproschema:ComputeSpecification a rdfs:Class ;
    rdfs:label "Compute Specification" ;
    rdfs:comment "An object to define computations in an activity or protocol." .

reproschema:DisableBack a rdfs:Class ;
    rdfs:label "Disable redo" ;
    rdfs:comment "Indicates (by boolean) if we can go back to a completed assessment in a protocol." .

reproschema:DontKnow a rdfs:Class ;
    rdfs:label "Do not know" ;
    rdfs:comment "An element to describe the choice when response is not known." .

reproschema:Field a nidm:DataElement,
        rdfs:Class,
        prov:Entity ;
    rdfs:label "Field" ;
    rdfs:comment "An item in an assessment." ;
    rdfs:subClassOf schema:CreativeWork .

reproschema:MessageSpecification a rdfs:Class ;
    rdfs:label "Message Specification" ;
    rdfs:comment "An object to define messages in an activity or protocol." .

reproschema:OverrideProperty a rdfs:Class ;
    rdfs:label "Additional properties" ;
    rdfs:comment "An object to override the various properties added to assessments and fields." .

reproschema:Participant a rdfs:Class,
        prov:Person ;
    rdfs:label "Participant" ;
    rdfs:comment "An Agent describing characteristics associated with a participant." ;
    rdfs:subClassOf prov:Agent .

reproschema:Protocol a rdfs:Class,
        prov:Entity,
        prov:Plan ;
    rdfs:label "Protocol" ;
    rdfs:comment "A representation of a study which comprises one or more assessments." ;
    rdfs:subClassOf schema:CreativeWork .

reproschema:Response a rdfs:Class,
        prov:Entity ;
    rdfs:label "Response" ;
    rdfs:comment "Describes the response of an item." ;
    rdfs:subClassOf schema:CreativeWork .

reproschema:ResponseActivity a rdfs:Class,
        prov:Activity ;
    rdfs:label "ResponseActivity" ;
    rdfs:comment "Captures information about some action that took place. It also links to information (entities) that were used during the activity" ;
    rdfs:subClassOf schema:CreativeWork .

reproschema:ResponseOption a rdfs:Class ;
    rdfs:label "Response option" ;
    rdfs:comment "An element (object or by URL)to describe the properties of response of the Field item." .

reproschema:Skipped a rdfs:Class ;
    rdfs:label "Skipped" ;
    rdfs:comment "An element to describe the choice when the item is skipped." .

reproschema:SoftwareAgent a rdfs:Class,
        prov:SoftwareAgent ;
    rdfs:label "Software Agent" ;
    rdfs:comment "Captures information about some action that took place. It also links to information (entities) that were used during the activity" .

reproschema:TimedOut a rdfs:Class ;
    rdfs:label "Response timed out" ;
    rdfs:comment "A boolean element to describe if the response did not occur within the prescribed time." .

reproschema:UnitOption a rdfs:Class ;
    rdfs:label "Unit options" ;
    rdfs:comment "An object to represent a human displayable name alongside the more formal value for units." .

nidm:subject_id rdfs:label "Participant identifier" ;
    schema:domainIncludes reproschema:Participant ;
    rdfs:comment "The identifier of a participant" .

schema:about a rdf:Property ;
    schema:domainIncludes reproschema:Activity,
        reproschema:Field,
        reproschema:Protocol ;
    rdfs:comment "The subject matter of the Field." .

schema:associatedMedia a rdf:Property ;
    rdfs:label "associatedMedia" ;
    schema:domainIncludes reproschema:Activity,
        reproschema:Field,
        reproschema:Protocol ;
    rdfs:comment "A media object that encodes this CreativeWork. This property is a synonym for encoding." .

schema:citation schema:domainIncludes reproschema:Activity .

schema:description schema:domainIncludes reproschema:Activity,
        reproschema:Field,
        reproschema:Protocol .

schema:image a rdf:Property ;
    rdfs:label "image" ;
    schema:domainIncludes reproschema:Choice,
        reproschema:Field ;
    rdfs:comment "An image of the item. This can be a <a class=\"localLink\" href=\"http://schema.org/URL\">URL</a> or a fully described <a class=\"localLink\" href=\"http://schema.org/ImageObject\">ImageObject</a>." .

schema:inLanguage schema:domainIncludes reproschema:ResponseActivity .

schema:isPartOf a rdf:Property ;
    schema:domainIncludes reproschema:Field ;
    schema:rangeIncludes reproschema:Activity .

schema:maxValue schema:domainIncludes reproschema:ResponseOption .

schema:minValue schema:domainIncludes reproschema:ResponseOption .

schema:name schema:domainIncludes reproschema:Choice .

schema:question a rdf:Property ;
    schema:domainIncludes reproschema:Field .

schema:readonlyValue a rdf:Property ;
    schema:domainIncludes reproschema:Field .

schema:schemaVersion a rdf:Property ;
    schema:domainIncludes reproschema:Activity,
        reproschema:Field,
        reproschema:Protocol .

schema:url schema:domainIncludes reproschema:SoftwareAgent .

schema:valueRequired schema:domainIncludes reproschema:AdditionalProperty,
        reproschema:OverrideProperty .

schema:version a rdf:Property ;
    schema:domainIncludes reproschema:Activity,
        reproschema:Field,
        reproschema:Protocol,
        reproschema:SoftwareAgent .

reproschema:addProperties a rdf:Property ;
    rdfs:label "addProperties" ;
    schema:domainIncludes reproschema:Activity,
        reproschema:Protocol ;
    schema:rangeIncludes reproschema:AdditionalProperty ;
    rdfs:comment "An array of objects to describe the various properties added to assessments and fields." .

reproschema:additionalNotesObj a rdf:Property ;
    rdfs:label "additional notes" ;
    schema:domainIncludes reproschema:Field ;
    schema:rangeIncludes reproschema:AdditionalNoteObj ;
    rdfs:comment "A set of objects to define notes in a field. For example, most Redcap and NDA data dictionaries have notes for each item which needs to be captured in reproschema." .

reproschema:allow a rdf:Property ;
    rdfs:label "allow" ;
    schema:domainIncludes reproschema:Activity,
        reproschema:Protocol ;
    schema:rangeIncludes schema:Thing ;
    rdfs:comment "An array of items indicating properties allowed on an activity or protocol " .

reproschema:choices a rdf:Property ;
    rdfs:label "choices" ;
    schema:domainIncludes reproschema:ResponseOption ;
    schema:rangeIncludes schema:URL,
        reproschema:Choice ;
    schema:sameAs schema:itemListElement ;
    rdfs:comment "An array to list the available options for response of the Field item." .

reproschema:column a rdf:Property ;
    rdfs:label "column" ;
    schema:domainIncludes reproschema:AdditionalNoteObj ;
    schema:rangeIncludes rdf:langString ;
    rdfs:comment "An element to define the column name where the note was taken from." .

reproschema:compute a rdf:Property ;
    rdfs:label "computation" ;
    schema:domainIncludes reproschema:Activity,
        reproschema:Protocol ;
    schema:rangeIncludes reproschema:ComputeSpecification ;
    rdfs:comment "An array of objects indicating computations in an activity or protocol and maps it to the corresponding Field item. scoring logic is a subset of all computations that could be performed and not all computations will be scoring. For example, one may want to do conversion from one unit to another. " .

reproschema:cronTable schema:domainIncludes reproschema:Activity,
        reproschema:Protocol .

reproschema:datumType a rdf:Property ;
    rdfs:label "datumType" ;
    schema:domainIncludes reproschema:ResponseOption ;
    schema:rangeIncludes schema:Text,
        schema:URL ;
    rdfs:comment "Indicates what type of datum the response is (e.g. range,count,scalar etc.) for the Field item." .

reproschema:inputType a rdf:Property ;
    rdfs:label "inputType" ;
    schema:domainIncludes reproschema:Field ;
    schema:rangeIncludes schema:Text ;
    rdfs:comment "An element to describe the input type of a Field item." .

reproschema:isAbout a rdf:Property ;
    rdfs:label "isAbout" ;
    schema:domainIncludes reproschema:AdditionalProperty,
        reproschema:OverrideProperty,
        reproschema:Response ;
    schema:rangeIncludes reproschema:Activity,
        reproschema:Field ;
    rdfs:comment "A pointer to the node describing the item." .

reproschema:isVis a rdf:Property ;
    rdfs:label "visibility" ;
    schema:domainIncludes reproschema:AdditionalProperty,
        reproschema:OverrideProperty ;
    schema:rangeIncludes schema:Boolean,
        schema:Text ;
    rdfs:comment "An element to describe (by boolean or conditional statement) visibility conditions of items in an assessment." .

reproschema:jsExpression a rdf:Property ;
    rdfs:label "JavaScript Expression" ;
    schema:domainIncludes reproschema:ComputeSpecification,
        reproschema:MessageSpecification ;
    schema:rangeIncludes schema:Boolean,
        schema:Text ;
    rdfs:comment "A JavaScript expression for computations.",
        "A JavaScript expression to compute a score from other variables." .

reproschema:landingPage a rdf:Property ;
    rdfs:label "Landing page content" ;
    schema:domainIncludes reproschema:Protocol ;
    schema:rangeIncludes schema:Text,
        schema:URL ;
    rdfs:comment "An element (by URL) to point to the protocol readme or landing page." .

reproschema:limit a rdf:Property ;
    rdfs:label "limit" ;
    schema:domainIncludes reproschema:AdditionalProperty,
        reproschema:OverrideProperty ;
    schema:rangeIncludes schema:Text ;
    rdfs:comment "An element to limit the duration (uses ISO 8601) this activity is allowed to be completed by once activity is available." .

reproschema:maxRetakes a rdf:Property ;
    rdfs:label "maxRetakes" ;
    schema:domainIncludes reproschema:AdditionalProperty,
        reproschema:OverrideProperty ;
    schema:rangeIncludes schema:Number ;
    rdfs:comment "Defines number of times the item is allowed to be redone." .

reproschema:message a rdf:Property ;
    rdfs:label "Message" ;
    schema:domainIncludes reproschema:MessageSpecification ;
    schema:rangeIncludes schema:Text,
        rdf:langString ;
    rdfs:comment "The message to be conditionally displayed for an item. " .

reproschema:messages a rdf:Property ;
    rdfs:label "messages" ;
    schema:domainIncludes reproschema:Activity,
        reproschema:Protocol ;
    schema:rangeIncludes reproschema:MessageSpecification ;
    rdfs:comment "An array of objects to define conditional messages in an activity or protocol." .

reproschema:multipleChoice a rdf:Property ;
    rdfs:label "Multiple choice response expectation" ;
    schema:domainIncludes reproschema:ResponseOption ;
    schema:rangeIncludes schema:Boolean ;
    rdfs:comment "Indicates (by bool) if response for the Field item has one or more answer." .

reproschema:order a rdf:Property ;
    rdfs:label "Order" ;
    schema:domainIncludes reproschema:Activity,
        reproschema:Protocol ;
    schema:rangeIncludes schema:URL,
        reproschema:Activity,
        reproschema:Field ;
    rdfs:comment "An ordered list to describe the order in which the items of an assessment or protocol appear in the user interface." .

reproschema:overrideProperties a rdf:Property ;
    rdfs:label "overrideProperties" ;
    schema:domainIncludes reproschema:Activity,
        reproschema:Protocol ;
    schema:rangeIncludes reproschema:OverrideProperty ;
    rdfs:comment "An array of objects to override the various properties added to assessments and fields." .

reproschema:preamble a rdf:Property ;
    rdfs:label "Preamble" ;
    schema:domainIncludes reproschema:Activity,
        reproschema:Field ;
    schema:rangeIncludes schema:Text,
        rdf:langString ;
    rdfs:comment "The preamble for an assessment" .

reproschema:randomMaxDelay a rdf:Property ;
    rdfs:label "randomMaxDelay" ;
    schema:domainIncludes reproschema:AdditionalProperty,
        reproschema:OverrideProperty ;
    schema:rangeIncludes schema:Text ;
    rdfs:comment "Present activity/item within some random offset of activity available time up to the maximum specified by this ISO 8601 duration" .

reproschema:responseOptions a rdf:Property ;
    rdfs:label "Response options" ;
    schema:domainIncludes reproschema:Field ;
    schema:rangeIncludes schema:URL,
        reproschema:ResponseOption ;
    rdfs:comment "An element (object or by URL)to describe the properties of response of the Field item." .

reproschema:schedule a rdf:Property ;
    rdfs:label "Schedule" ;
    schema:domainIncludes reproschema:AdditionalProperty,
        reproschema:OverrideProperty ;
    schema:rangeIncludes schema:Schedule,
        schema:Text ;
    rdfs:comment "An element to set make activity available/repeat info using ISO 8601 repeating interval format." .

reproschema:shuffle a rdf:Property ;
    rdfs:label "Shuffle" ;
    schema:domainIncludes reproschema:Activity,
        reproschema:Protocol ;
    schema:rangeIncludes schema:boolean ;
    rdfs:comment "An element (bool) to determine if the list of items is shuffled or in order." .

reproschema:source a rdf:Property ;
    rdfs:label "source" ;
    schema:domainIncludes reproschema:AdditionalNoteObj ;
    schema:rangeIncludes rdf:langString ;
    rdfs:comment "An element to define the source (eg. RedCap, NDA) where the note was taken from." .

reproschema:statusOptions a rdf:Property ;
    rdfs:label "Status options" ;
    schema:rangeIncludes schema:Text ;
    rdfs:comment "Provides information on whether or not a field item wants to be accompanied by the additional status option(s) defined in “statusOptions”" .

reproschema:unitOptions a rdf:Property ;
    rdfs:label "unitOptions" ;
    schema:domainIncludes reproschema:ResponseOption ;
    schema:rangeIncludes reproschema:UnitOption ;
    rdfs:comment "A list of objects to represent a human displayable name alongside the more formal value for units." .

reproschema:value a rdf:Property ;
    rdfs:label "value" ;
    schema:domainIncludes reproschema:AdditionalNoteObj,
        reproschema:UnitOption ;
    schema:rangeIncludes schema:Boolean,
        schema:Number,
        schema:StructuredValue,
        schema:Text,
        schema:URL ;
    schema:sameAs schema:value ;
    rdfs:comment "The value for each option in choices or in additionalNotesObj" .

reproschema:valueType a rdf:Property ;
    rdfs:label "The type of the response" ;
    schema:domainIncludes reproschema:ResponseOption ;
    schema:rangeIncludes schema:Text,
        rdf:langString ;
    rdfs:comment "The type of the response of an item. For example, string, integer, etc." .

reproschema:variableName a rdf:Property ;
    rdfs:label "variableName" ;
    schema:domainIncludes reproschema:AdditionalProperty,
        reproschema:ComputeSpecification,
        reproschema:OverrideProperty ;
    schema:rangeIncludes schema:Text ;
    rdfs:comment "The name used to represent an item." .

skos:altLabel a rdf:Property ;
    rdfs:label "alternate label" ;
    schema:domainIncludes reproschema:Activity,
        reproschema:Field,
        reproschema:Protocol ;
    schema:rangeIncludes schema:Text ;
    rdfs:comment "The alternate label." .

skos:prefLabel a rdf:Property ;
    rdfs:label "preferred label" ;
    schema:domainIncludes reproschema:Activity,
        reproschema:AdditionalProperty,
        reproschema:Field,
        reproschema:OverrideProperty,
        reproschema:Protocol,
        reproschema:UnitOption ;
    schema:rangeIncludes schema:Text ;
    rdfs:comment "The preferred label." .

prov:endedAtTime schema:domainIncludes reproschema:ResponseActivity .

prov:generated schema:domainIncludes reproschema:ResponseActivity .

prov:startedAtTime schema:domainIncludes reproschema:ResponseActivity .

prov:used schema:domainIncludes reproschema:ResponseActivity .

prov:wasAttributedTo schema:domainIncludes reproschema:Response ;
    schema:rangeIncludes reproschema:Participant .

schema:value schema:domainIncludes reproschema:Choice,
        reproschema:Response ;
    schema:rangeIncludes schema:Boolean,
        schema:Number,
        schema:StructuredValue,
        schema:Text,
        schema:URL,
        reproschema:DontKnow,
        reproschema:Skipped .
